Implement qop and 4 storage for 4 blood types

inventory.dfy
@@ -1,5 +1,6 @@
 include "bloodRep.dfy"
 module inventory {
+    import BR = BloodRep
     class Quack<Data>
     {
         var buf: array<Data>
@@ -72,11 +73,113 @@ module inventory {
             shadow := shadow + [x];
         }
 
+        method HeadTail()
+        modifies this, this.buf;
+        requires buf!=null
+        requires shadow != [];
+        requires Valid(); ensures Valid();
+        ensures |shadow| == old(|shadow|)
+        ensures |shadow| > 1 ==> shadow == [old(shadow[|old(shadow)|-1])] + old(shadow[1..|old(shadow)|-1]) + [old(shadow[0])]
+        ensures |shadow| <= 1 ==> shadow == old(shadow)
+        ensures buf == old(buf)
+        {
+            buf[m], buf[n-1] := buf[n-1],buf[m];
+            if(|shadow| > 1)
+            {
+                shadow := [shadow[|shadow|-1]] + shadow[1..|shadow|-1] + [shadow[0]];
+            } 
+        }   
+
     }
 
     class Inventory
     {
-        
+        var A : Quack<BR.BloodRecord>;
+        var B : Quack<BR.BloodRecord>;
+        var AB : Quack<BR.BloodRecord>;
+        var O : Quack<BR.BloodRecord>;
+
+        /*
+         * Valid() to make sure that A,B,AB,O are instantiated 
+         */
+        predicate Valid()
+        reads this, this.A, this.B, this.AB, this.O
+        {
+            A != null && A.buf != null && A.buf.Length != 0 &&
+            B != null && B.buf != null && B.buf.Length != 0 &&
+            AB != null && AB.buf != null && AB.buf.Length != 0 &&
+            O != null && O.buf != null && O.buf.Length != 0
+        }
+
+        /*
+         * to make sure that the groups are grouped correctly
+         */
+        predicate ValidGroup()
+        requires Valid()
+        reads this, this.A, this.A.buf, this.B, this.B.buf ,this.AB, this.AB.buf ,this.O, this.O.buf;
+        { 
+            (forall i :: 0 <= A.m <= i < A.n <= A.buf.Length ==> A.buf[i].bType == BR.BloodType.A) &&
+            (forall i :: 0 <= B.m <= i < B.n <= B.buf.Length ==> B.buf[i].bType == BR.BloodType.B) &&
+            (forall i :: 0 <= AB.m <= i < AB.n <= AB.buf.Length ==> AB.buf[i].bType == BR.BloodType.AB) &&
+            (forall i :: 0 <= O.m <= i < O.n <= O.buf.Length ==> O.buf[i].bType == BR.BloodType.O)
+        }
+
+        constructor() modifies this
+        ensures fresh(A) && fresh(B) && fresh(AB) && fresh(O);
+        ensures A.buf != null && A.buf.Length != 0;
+        ensures B.buf != null && B.buf.Length != 0;
+        ensures AB.buf != null && AB.buf.Length != 0;
+        ensures O.buf != null && O.buf.Length != 0;
+        ensures Valid() && ValidGroup();
+        {
+            A := new Quack(1); assert A.buf != null && A.buf.Length != 0;
+            B := new Quack(1); assert B.buf != null && B.buf.Length != 0;
+            AB := new Quack(1); assert AB.buf != null && AB.buf.Length != 0;
+            O := new Quack(1); assert O.buf != null && O.buf.Length != 0;
+        }
+        method Empty(t:BR.BloodType) returns (x:bool)
+        modifies this.A, this.B, this.AB, this.O;
+        requires Valid() && ValidGroup();ensures Valid()&& ValidGroup();
+        requires A.Valid() && B.Valid() && AB.Valid() && O.Valid(); ensures A.Valid() && B.Valid() && AB.Valid() && O.Valid();
+        {
+            match (t)
+            {
+                case A => x:= this.A.Empty();
+                case B => x:= this.B.Empty();
+                case AB => x:= this.AB.Empty();
+                case O => x:= this.O.Empty();
+            }
+        }
+        method Pop(t:BR.BloodType) returns(x: BR.BloodRecord) modifies this, this`A, this`B, this`AB, this`O
+        requires Valid() && ValidGroup();ensures Valid() && ValidGroup();
+        requires A.Valid() && B.Valid() && AB.Valid() && O.Valid(); ensures A.Valid() && B.Valid() && AB.Valid() && O.Valid();
+        modifies this.A, this.B, this.AB, this.O
+
+        method Qop(t:BR.BloodType) returns (x: BR.BloodRecord) modifies this, this`A, this`B, this`AB, this`O
+        requires Valid() && ValidGroup();ensures Valid()&& ValidGroup();
+        requires A.Valid() && B.Valid() && AB.Valid() && O.Valid(); ensures A.Valid() && B.Valid() && AB.Valid() && O.Valid();
+
+        method Push(t:BR.BloodType, x:BR.BloodRecord) modifies this, this`A, this`B, this`AB, this`O
+        requires Valid() && ValidGroup();ensures Valid()&& ValidGroup();
+        requires A.Valid() && B.Valid() && AB.Valid() && O.Valid(); ensures A.Valid() && B.Valid() && AB.Valid() && O.Valid();
+        requires t == BR.BloodType.A <==> x.bType == BR.BloodType.A;
+        requires t == BR.BloodType.B <==> x.bType == BR.BloodType.B;
+        requires t == BR.BloodType.AB <==> x.bType == BR.BloodType.AB;
+        requires t == BR.BloodType.O <==> x.bType == BR.BloodType.O;
+        //{
+        //    match (t)
+        //    {
+        //        case A => this.A.Push(x);
+        //        case B => this.B.Push(x);
+        //        case AB => this.AB.Push(x);
+        //        case O => this.O.Push(x);
+        //    }
+        //}
+
+
+        method HeadTail()
+        requires Valid() && ValidGroup();ensures Valid()&& ValidGroup();
+        requires A.Valid() && B.Valid() && AB.Valid() && O.Valid(); ensures A.Valid() && B.Valid() && AB.Valid() && O.Valid();
     }
 
 }
